\documentclass{article}
\usepackage{graphicx, amsmath, amssymb, mathtools, fancyhdr}

\setlength{\oddsidemargin}{0in}
\setlength{\textwidth}{6.5in}
\setlength{\topmargin}{-.55in}
\setlength{\textheight}{9in}
\pagestyle{fancy}

\fancyfoot{}
\fancyhead[R]{\thepage}
\fancyhead[L]{MATH }


\begin{document}

\begin{center}
    {\huge Nonlinear Waves Problem 4.1}
    \vspace{0.5cm}

    {\large Michael Nameika}
\end{center}

4.1
\begin{itemize}
    \item[(a)] Obtain the nonlinear change in the frequency given by (4.19) by applying the frequency-shift method to the equation
    \[\frac{d^2y}{dt^2} + y - \varepsilon y^3 = 0, \hspace{0.5cm} |\varepsilon| \ll 1.\]
    \textit{Soln.} Introduce the new time variable $\tau  = \omega t$ so that $\frac{d}{dt} = \omega \frac{d}{d\tau}$. Then the ODE becomes
    \[\omega^2\frac{dy^2}{d\tau^2} + y - \varepsilon y^3 = 0.\]
    Assume that $y = y_0 + \varepsilon y_1 + \varepsilon^2y_2 + \cdots$ and $\omega = 1 + \varepsilon\omega_1 + \varepsilon^2\omega_2 + \cdots$. Plugging this into the differential equation yields
    \begin{align*}
        (1 + \varepsilon \omega_1 + \cdots)^2\frac{d}{d\tau}(y_0 + \varepsilon y_1 + \varepsilon^2y_2 + \cdots) + y_0 + \varepsilon y_1 + \varepsilon^2y_2 + \cdots - \varepsilon(y_0 + \varepsilon y_1 + \varepsilon^2y_2 + \cdots)^3 &= 0.
    \end{align*}
    Collecting the order 1 and $\varepsilon$ terms gives
    \begin{align*}
        \mathcal{O}(1): \hspace{0.5cm} &y_0'' + y_0 = 0\\
        \implies &y_0  = A e^{i\tau} + \text{c.c.}\\
        \mathcal{O}(\varepsilon): \hspace{0.5cm} &y_1'' + \omega_1y_0'' + y_1 - y_0^3 = 0\\
        \implies &y_1'' + y_1 = 2\omega_1Ae^{i\tau} + 3A^2A^*e^{i\tau} + A^3e^{3i\tau} + \text{c.c.}
    \end{align*}
    For the $\mathcal{O}(\varepsilon)$ equation, notice the secular terms are $2\omega_1e^{i\tau} + 3A^2A^*e^{i\tau}$, so we make the restriction
    \begin{align*}
        2\omega_1A + 3A^2A^* &= 0\\
        \implies \omega_1 = -\frac{3}{2}|A|^2.
    \end{align*}
    And for $y_1$, we wish to solve the equation
    \[y_1'' + y_1 = A^3e^{3i\tau} + \text{c.c.}\]
    Using the ansatz $y_1 = Be^{3i\tau} + \text{c.c.}$, we find
    \begin{align*}
        -8Be^{3i\tau} + \text{c.c.} &= A^3e^{3i\tau} + \text{c.c.}\\
        \implies B &= -\frac{A^3}{8}
    \end{align*}
    and so
    \[y_1 = -\frac{A^3}{8}e^{3i\tau} + \text{c.c.}\]
    Putting it together, we have
    \[y \sim Ae^{it\left(1 - \frac{3}{2}|A|^2\right)} - \varepsilon\frac{A^3}{8}e^{3it\left(1 - \frac{3}{2}|A|^2\right)} + \text{c.c.}\]
    and so we find the nonlinear change in the frequency is given by
    \[\Omega = 1 - \frac{3}{2}|A|^2\]
    as desired.

    \item[(b)] Use the multiple-scales method to find the leading-order approximation to the solution of 
    \[\frac{d^2y}{dt^2} + y -\varepsilon\left(y^3 + \frac{dy}{dt}\right) = 0, \hspace{0.5cm} 0 < \varepsilon \ll 1.\]
    \textit{Soln.} See part (c).

    \item[(c)] Find the next-order (first-order) approximation, valid for times $t = o(1/\varepsilon^2),$ to the solution of part (b).
    \newline\newline
    \textit{Soln.} Since we need to find the leading-order behavior to find the first-order approximation, we complete part (b) here. Introduce the fast time and slow time variables $t_1 = t$ and $t_2 = \varepsilon t$. Via the chain rule, we find
    \[\frac{d}{dt} = \frac{\partial}{\partial t_1} + \varepsilon\frac{\partial}{\partial t_2}.\]
    We also assume $y = y_0 + \varepsilon y_1 + \varepsilon^2 y_2 + \cdots$ and plugging these into the differential equation given in part (b) gives
    \begin{align*}
        &\left(\frac{\partial}{\partial t_1} + \varepsilon\frac{\partial}{\partial t_2}\right)^2(y_0 + \varepsilon y_1 + \varepsilon^2y_2 + \cdots) + y_0 + \varepsilon y_1 + \varepsilon^2y_2 + \cdots +\\
        &-\varepsilon\left((y_0 + \varepsilon y_1 + \varepsilon^2y_2)^3 + \left(\frac{\partial}{\partial t_1} + \varepsilon\frac{\partial}{\partial t_2}\right)(y_0 + \varepsilon y_1 + \varepsilon^2y_2 + \cdots)\right) = 0
    \end{align*}
    which yields, to $\mathcal{O}(\varepsilon)$:
    \[\frac{\partial^2y_1}{\partial t_1^2} + 2\frac{\partial^2y_0}{\partial t_1\partial t_2} + y_1 - y_0^3 - \frac{\partial y_0}{\partial t_1} = 0.\]
    Solving the $\mathcal{O}(1)$ and $\mathcal{O}(\varepsilon)$:
    \begin{align*}
        \mathcal{O}(1): \hspace{0.5cm} &\frac{\partial^2y_0}{\partial t_1^2} + y_0 = 0\\
        \implies &y_0 = A(t_2)e^{i2_1} + \text{c.c.}\\
        \mathcal{O}(\varepsilon): \hspace{0.5cm} &\frac{\partial^2y_1}{\partial t_1^2} + 2\frac{\partial^2y_0}{\partial t_1\partial t_2} + y_1 - y_0^3 - \frac{\partial y_0}{\partial t+1} = 0\\
        \implies &\frac{\partial^2y_1}{\partial t_1^2} + y_1 = A^3e^{3it_1} + A^2A^*e^{it_1} + iAe^{it_1} - 2iA'e^{it_1} + \text{c.c.}
    \end{align*}
    In the above differential equation for $y_1$, note that the secular term on the right hand side are $e^{it_1}(A^2A^* + iA - 2iA')$ and so we set the secular term to zero:
    \begin{align*}
        &A^2A^* + iA - 2iA' = 0\\
        \implies &2iA' - iA= A|A|^2
    \end{align*}
    multiplying by $A^*$ yields
    \begin{align*}
        &2iA'A^* - i|A|^2 = |A|^4 \in \mathbb{R}\\
        \implies &2iA'A^* + 2i(A')^*A - 2i|A|^2 = 0\\
        \implies &\frac{d}{dt_2}\left(|A|^2\right) = |A|^2\\
        \implies &|A(t_2)|^2 = Ce^{t_2}
    \end{align*}
    where $C$ is a constant of integration. For $t_2 = 0$, $|A(0)|^2 = C$, so call $C = |A_0|^2$. Thus
    \[|A(t_2)|^2 = |A_0|^2e^{t_2}.\]
    By our choice of $A$, we have the differential equation for $y_1$ becomes
    \[\frac{\partial^2y_1}{\partial t_1^2} + y_1 = A^3e^{3it_1} + \text{c.c.}\]
    and using the ansatz $y_1 = Be^{3it_1} + \text{c.c.}$ yields $B = -A^3/8$ and so
    \[y_1 = -\frac{A^3}{8}e^{3it_1} + \text{c.c.}\]
    Now let us find a more explicit formula for $A(t_2)$. From the differential equation for $A$,
    \begin{align*}
        2iA' &= |A|^2A + iA\\
        \implies 2iA' &= |A_0|^2e^{t_2}A + iA\\
        \implies 2iA' &= A\left(|A_0|^2e^{t_2} + i\right)\\
        \implies A' &= A\left(-\frac{i}{2}|A|_0^2e^{t_2} + \frac{1}{2}\right)\\
        \implies A &= Ce^{\left(t_2/2 - i/2|A_0|^2e^{t_2}\right)}
    \end{align*}
    and using $A(0) = A_0$, we have $C = A_0e^{i/2|A_0|^2}$ and so
    \begin{align*}
        A(t_2) &= A_0e^{t2/2}e^{i/2\left(|A_0|^2(1 - e^{t_2})\right)}.
    \end{align*}
    Putting it together, we have
    \[y \sim A_0e^{\varepsilon t/2}e^{i/2|A_0|^2(1 - e^{\varepsilon t}) + it} - \varepsilon \frac{A_0^3}{8}e^{3/2\varepsilon t}e^{3i/2|A_0|^2(1 - e^{\varepsilon t}) + 3it} + \text{c.c.}\]
\end{itemize}

\end{document}
